Make SMTLib semantics dependently-typed and total
Squashed commits:
- Add proof of no zero-width vars in Verilog syntax
- Add some useful metatheory about whole modules (requires sortable)
- Fix up proof for dependent SMTLIB

vera/SMTQueries.v
@@ -7,15 +7,14 @@ From Stdlib Require Import Morphisms.
 
 From vera Require Import Tactics.
 From vera Require Import Common.
-From vera Require SMTLib.
+From vera Require Import SMTLib.
+From vera Require Import Bitvector.
 
 Import ListNotations.
 
-Fixpoint term_domain (t : SMTLib.term) : list SMTLib.const_sym :=
+Fixpoint term_domain {s} (t : term s) : list const_sym :=
   match t with
-  | SMTLib.Term_Const sym => [sym]
-  | SMTLib.Term_Int _ => []
-  | SMTLib.Term_Geq l r => term_domain l ++ term_domain r
+  | SMTLib.Term_Const _ sym => [sym]
   | SMTLib.Term_Eq l r => term_domain l ++ term_domain r
   | SMTLib.Term_And l r => term_domain l ++ term_domain r
   | SMTLib.Term_Or l r => term_domain l ++ term_domain r
@@ -25,152 +24,105 @@ Fixpoint term_domain (t : SMTLib.term) : list SMTLib.const_sym :=
   | SMTLib.Term_False => []
   | SMTLib.Term_BVLit _ _ => []
   | SMTLib.Term_BVConcat l r => term_domain l ++ term_domain r
-  | SMTLib.Term_BVExtract _ _ e => term_domain e
+  | SMTLib.Term_BVExtract _ _ _ e => term_domain e
   | SMTLib.Term_BVUnaryOp _ e => term_domain e
   | SMTLib.Term_BVBinOp _ l r => term_domain l ++ term_domain r
   | SMTLib.Term_BVUlt l r => term_domain l ++ term_domain r
   end
 .
 
-Definition lst_domain (q : list SMTLib.term) : list SMTLib.const_sym :=
+Definition lst_domain {s} (q : list (term s)) : list const_sym :=
   List.concat (List.map term_domain q).
 
 Definition declaration := (nat * SMTLib.sort)%type.
 
-Record query :=
-  MkQuery
-    {
-      declarations : list declaration;
-      assertions : list SMTLib.term;
-      (* All constants used have been declared *)
-      wf : Forall
-             (fun n => exists s, In (n, s) declarations)
-             (lst_domain assertions)
-    }.
+Definition query := list (term (Sort_Bool)).
 
-Record decl_term :=
-  MkDeclTerm
-    {
-      dtDeclarations : list declaration;
-      dtTerm : SMTLib.term;
-      (* All constants used have been declared *)
-      dtWf : Forall
-             (fun n => exists s, In (n, s) dtDeclarations)
-             (term_domain dtTerm)
-    }.
+Definition domain (q : query) : list const_sym := lst_domain q.
 
-Definition domain (q : query) : list SMTLib.const_sym := lst_domain (assertions q).
-
-Definition valuation := nat -> option SMTLib.value.
-
-Definition valuation_set_fun (ρ : valuation) (n : nat) (v : SMTLib.value) : valuation :=
-  fun n' => if n =? n' then Some v else ρ n.
-
-Hint Unfold valuation_set_fun : core.
-
-Definition default_valuation : valuation := fun _ => None.
-
-Inductive value_has_sort : SMTLib.value -> SMTLib.sort -> Prop :=
-| value_has_sort_Bool b : value_has_sort (SMTLib.Value_Bool b) SMTLib.Sort_Bool
-| value_has_sort_Int i : value_has_sort (SMTLib.Value_Int i) SMTLib.Sort_Int
-| value_has_sort_BitVec w bv : value_has_sort (SMTLib.Value_BitVec w bv) (SMTLib.Sort_BitVec w)
+Definition default_valuation : valuation := fun s _ =>
+  match s with
+  | Sort_Bool => false
+  | Sort_BitVec w => BV.zeros w
+  end
 .
 
-Definition valuation_matches_decls (ρ: valuation) (ds: list declaration) : Prop :=
-  Forall (fun '(n, s) => exists v, ρ n = Some v /\ value_has_sort v s) ds.
-
-Definition term_satisfied_by (ρ: valuation) (t: SMTLib.term) : Prop :=
-    SMTLib.interp_term ρ t = Some (SMTLib.Value_Bool true).
-
-Definition decl_term_satisfied_by (ρ: valuation) (t: decl_term) : Prop :=
-  valuation_matches_decls ρ (dtDeclarations t) /\
-    term_satisfied_by ρ (dtTerm t).
+Definition term_satisfied_by (ρ: SMTLib.valuation) (t: SMTLib.term Sort_Bool) : Prop :=
+  SMTLib.interp_term ρ t = true.
 
 Definition satisfied_by (ρ: valuation) (q: query): Prop :=
-  valuation_matches_decls ρ (declarations q) /\
-    Forall (term_satisfied_by ρ) (assertions q).
+  Forall (term_satisfied_by ρ) q.
 
-Lemma decl_term_app_wf t1 t2:
-  Forall (fun n : nat => exists s : SMTLib.sort, In (n, s) (dtDeclarations t1 ++ dtDeclarations t2))
-    (term_domain (dtTerm t1) ++ term_domain (dtTerm t2)).
-Proof.
-  destruct t1, t2. simpl.
-  apply Forall_app.
-  rewrite ! Forall_forall in *.
-  split; intros.
-  - edestruct dtWf0; eauto.
-    eexists. apply List.in_app_iff.
-    eauto.
-  - edestruct dtWf1; eauto.
-    eexists. apply List.in_app_iff.
-    eauto.
-Qed.
+(* Definition decl_term_satisfied_by (ρ: valuation) (t: decl_term) : Prop :=
+ *   valuation_matches_decls ρ (dtDeclarations t) /\
+ *     term_satisfied_by ρ (dtTerm t).
+ * 
+ * 
+ * Lemma decl_term_app_wf t1 t2:
+ *   Forall (fun n : nat => exists s : SMTLib.sort, In (n, s) (dtDeclarations t1 ++ dtDeclarations t2))
+ *     (term_domain (dtTerm t1) ++ term_domain (dtTerm t2)).
+ * Proof.
+ *   destruct t1, t2. simpl.
+ *   apply Forall_app.
+ *   rewrite ! Forall_forall in *.
+ *   split; intros.
+ *   - edestruct dtWf0; eauto.
+ *     eexists. apply List.in_app_iff.
+ *     eauto.
+ *   - edestruct dtWf1; eauto.
+ *     eexists. apply List.in_app_iff.
+ *     eauto.
+ * Qed.
+ * 
+ * Definition not_decl_term (t : decl_term) : decl_term :=
+ *   {|
+ *     dtDeclarations := dtDeclarations t;
+ *     dtTerm := SMTLib.Term_Not (dtTerm t);
+ *     dtWf := dtWf t
+ *   |}
+ * .
+ * 
+ * Definition and_decl_term (t1 t2 : decl_term) : decl_term :=
+ *   {|
+ *     dtDeclarations := dtDeclarations t1 ++ dtDeclarations t2;
+ *     dtTerm := SMTLib.Term_And (dtTerm t1) (dtTerm t2);
+ *     dtWf := decl_term_app_wf t1 t2
+ *   |}
+ * .
+ * 
+ * Definition or_decl_term (t1 t2 : decl_term) : decl_term :=
+ *   {|
+ *     dtDeclarations := dtDeclarations t1 ++ dtDeclarations t2;
+ *     dtTerm := SMTLib.Term_Or (dtTerm t1) (dtTerm t2);
+ *     dtWf := decl_term_app_wf t1 t2
+ *   |}
+ * . *)
 
-Definition not_decl_term (t : decl_term) : decl_term :=
-  {|
-    dtDeclarations := dtDeclarations t;
-    dtTerm := SMTLib.Term_Not (dtTerm t);
-    dtWf := dtWf t
-  |}
-.
-
-Definition and_decl_term (t1 t2 : decl_term) : decl_term :=
-  {|
-    dtDeclarations := dtDeclarations t1 ++ dtDeclarations t2;
-    dtTerm := SMTLib.Term_And (dtTerm t1) (dtTerm t2);
-    dtWf := decl_term_app_wf t1 t2
-  |}
-.
-
-Definition or_decl_term (t1 t2 : decl_term) : decl_term :=
-  {|
-    dtDeclarations := dtDeclarations t1 ++ dtDeclarations t2;
-    dtTerm := SMTLib.Term_Or (dtTerm t1) (dtTerm t2);
-    dtWf := decl_term_app_wf t1 t2
-  |}
-.
-
-Definition term_reflect_if
-  (C : valuation -> Prop)
-  (t: SMTLib.term)
+Definition term_reflect
+  (t: term Sort_Bool)
   (P : valuation -> Prop) : Prop :=
-  forall ρ, C ρ -> term_satisfied_by ρ t <-> P ρ.
-
-Definition term_reflect := term_reflect_if (fun _ => True).
+  forall ρ, term_satisfied_by ρ t <-> P ρ.
 
 Global Typeclasses Transparent term_reflect.
 
-Global Instance term_reflect_if_proper :
+Global Instance term_reflect_proper :
   Proper
-    (pointwise_relation valuation iff ==> eq ==> pointwise_relation valuation iff ==> iff)
-    term_reflect_if.
+    (eq ==> pointwise_relation valuation iff ==> iff)
+    term_reflect.
 Proof.
   unfold
     pointwise_relation,
-    term_reflect_if.
+    term_reflect.
   repeat intro.
   setoid_rewrite H.
   setoid_rewrite H0.
-  setoid_rewrite H1.
   reflexivity.
 Qed.
 
-Lemma term_reflect_if_elim C t P :
-  term_reflect_if C t P ->
-  (forall ρ, P ρ -> C ρ) ->
-  (forall ρ, term_satisfied_by ρ t -> C ρ) ->
-  term_reflect t P.
-Proof. unfold term_reflect_if. firstorder. Qed.
-
-Lemma term_reflect_if_intro C t P :
-  term_reflect t P ->
-  term_reflect_if C t P.
-Proof. unfold term_reflect_if. firstorder. Qed.
-
-Lemma term_reflect_iff t C P1 P2 :
+Lemma term_reflect_iff t P1 P2 :
   (pointwise_relation _ iff P1 P2) ->
-  term_reflect_if C t P1 ->
-  term_reflect_if C t P2.
+  term_reflect t P1 ->
+  term_reflect t P2.
 Proof.
   intros H Hreflect.
   setoid_rewrite <- H.
@@ -182,14 +134,16 @@ Lemma term_reflect_and q1 q2 P1 P2 :
   term_reflect q2 P2 ->
   term_reflect (SMTLib.Term_And q1 q2) (fun ρ => P1 ρ /\ P2 ρ).
 Proof.
-  unfold term_reflect, term_reflect_if, term_satisfied_by.
+  unfold term_reflect, term_satisfied_by.
   intros Hrefl1 Hrefl2.
   simpl.
-  intros ρ _.
+  intros ρ.
   split; intros * H.
-  - autodestruct_eqn E.
-    Bool.destr_bool.
-    crush.
+  - rewrite <- Hrefl1 by trivial.
+    rewrite <- Hrefl2 by trivial.
+    generalize dependent (interp_term ρ q1); intro b1; intros.
+    generalize dependent (interp_term ρ q2); intro b2; intros.
+    now repeat Bool.destr_bool.
   - setoid_rewrite <- Hrefl1 in H; trivial; [].
     setoid_rewrite <- Hrefl2 in H; trivial; [].
     destruct H as [H1 H2].
@@ -197,33 +151,19 @@ Proof.
     reflexivity.
 Qed.
 
-Lemma term_reflect_or C1 C2 q1 q2 P1 P2 :
-  term_reflect_if C1 q1 P1 ->
-  term_reflect_if C2 q2 P2 ->
-  term_reflect_if
-    (fun ρ =>
-       (exists b, SMTLib.interp_term ρ q1 = Some (SMTLib.Value_Bool b))
-       /\ (exists b, SMTLib.interp_term ρ q2 = Some (SMTLib.Value_Bool b))
-       /\ C1 ρ
-       /\ C2 ρ
-    )
-    (SMTLib.Term_Or q1 q2)
-    (fun ρ => P1 ρ \/ P2 ρ).
+Lemma term_reflect_or q1 q2 P1 P2 :
+  term_reflect q1 P1 ->
+  term_reflect q2 P2 ->
+  term_reflect (SMTLib.Term_Or q1 q2) (fun ρ => P1 ρ \/ P2 ρ).
 Proof.
-  unfold term_reflect, term_reflect_if, term_satisfied_by.
+  unfold term_reflect, term_reflect, term_satisfied_by.
   simpl.
-  intros Hrefl1 Hrefl2 ρ [[b1 Hb1] [[b2 Hb2] [HC1 HC2]]].
-  specialize (Hrefl1 ρ ltac:(trivial)).
-  specialize (Hrefl2 ρ ltac:(trivial)).
-  rewrite Hb1, Hb2 in *. clear Hb1 Hb2.
-  split; intros * H.
-  - inv H.
-    Bool.destr_bool; crush.
-  - setoid_rewrite <- Hrefl1 in H; trivial; [].
-    setoid_rewrite <- Hrefl2 in H; trivial; [].
-    destruct H as [H|H];
-      inv H;
-      Bool.destr_bool.
+  intros Hrefl1 Hrefl2 ρ.
+  specialize (Hrefl1 ρ).
+  specialize (Hrefl2 ρ).
+  rewrite Bool.orb_true_iff.
+  rewrite Hrefl1, Hrefl2.
+  reflexivity.
 Qed.
 
 Definition satisfiable (q: query) : Prop :=
@@ -258,72 +198,22 @@ Qed.
 
 Infix "⊧" := satisfied_by (at level 20).
 
-Definition smt_reflect_if (C: valuation -> Prop) (q: query) (P : valuation -> Prop): Prop :=
-  forall ρ, C ρ -> ρ ⊧ q <-> P ρ.
-
-Definition smt_reflect := smt_reflect_if (fun _ => True).
-
-Global Instance smt_reflect_if_proper :
-  Proper
-    (pointwise_relation valuation iff ==> eq ==> pointwise_relation valuation iff ==> iff)
-    smt_reflect_if.
-Proof.
-  unfold
-    pointwise_relation,
-    smt_reflect_if.
-  repeat intro.
-  setoid_rewrite H.
-  setoid_rewrite H0.
-  setoid_rewrite H1.
-  reflexivity.
-Qed.
+Definition smt_reflect (q: query) (P : valuation -> Prop): Prop :=
+  forall ρ, ρ ⊧ q <-> P ρ.
 
 Global Instance smt_reflect_proper :
   Proper
     (eq ==> pointwise_relation valuation iff ==> iff)
     smt_reflect.
-Proof. unfold smt_reflect. typeclasses eauto. Qed.
-
-Lemma smt_reflect_if_elim C t P :
-  smt_reflect_if C t P ->
-  (forall ρ, P ρ -> C ρ) ->
-  (forall ρ, satisfied_by ρ t -> C ρ) ->
-  smt_reflect t P.
-Proof. unfold smt_reflect_if. firstorder. Qed.
-
-Lemma smt_reflect_if_intro C t P :
-  smt_reflect t P ->
-  smt_reflect_if C t P.
-Proof. unfold smt_reflect_if. firstorder. Qed.
-
-Lemma combine_wf q1 q2 :
-  List.Forall
-    (fun n : nat => exists s : SMTLib.sort, List.In (n, s) (declarations q1 ++ declarations q2))
-    (lst_domain (assertions q1 ++ assertions q2)).
 Proof.
-  destruct q1, q2.
-  unfold lst_domain in *.
-  rewrite ! List.Forall_forall in *.
-  simpl in *.
-  rewrite List.Forall_forall in *.
-  intros n H.
-  rewrite
-    <- List.flat_map_concat_map,
-    List.flat_map_app,
-    List.in_app_iff
-    in *.
-  setoid_rewrite List.in_app_iff.
-  destruct H.
-  - edestruct wf0 as [n' Hwf]; eauto.
-  - edestruct wf1 as [n' Hwf]; eauto.
+  unfold pointwise_relation, smt_reflect.
+  repeat intro.
+  setoid_rewrite H.
+  setoid_rewrite H0.
+  reflexivity.
 Qed.
 
-Definition combine (q1 q2: query) : query :=
-  {|
-    declarations := declarations q1 ++ declarations q2;
-    assertions := assertions q1 ++ assertions q2;
-    wf := combine_wf q1 q2
-  |}.
+Definition combine (q1 q2: query) : query := q1 ++ q2.
 
 Lemma concat_conj :
   forall q1 q2 P1 P2,
@@ -331,96 +221,64 @@ Lemma concat_conj :
     smt_reflect q2 P2 ->
     smt_reflect (combine q1 q2) (fun ρ => P1 ρ /\ P2 ρ).
 Proof.
-  destruct q1, q2.
-  unfold smt_reflect, smt_reflect_if, satisfied_by, combine.
+  unfold smt_reflect, satisfied_by, combine.
   simpl.
   intros.
   setoid_rewrite List.Forall_app.
   firstorder.
 Qed.
 
-Lemma lst_domain_app xs ys :
-  lst_domain (xs ++ ys) = lst_domain xs ++ lst_domain ys.
+Lemma lst_domain_app s xs ys :
+  @lst_domain s (xs ++ ys) = lst_domain xs ++ lst_domain ys.
 Proof.
   unfold lst_domain.
   now rewrite List.map_app, List.concat_app.
 Qed.
 
-Lemma lst_domain_cons x xs :
-  lst_domain (x :: xs) = term_domain x ++ lst_domain xs.
+Lemma lst_domain_cons s x xs :
+  @lst_domain s (x :: xs) = term_domain x ++ lst_domain xs.
 Proof. reflexivity. Qed.
 
-Program Definition add_assertion
-  (a : SMTLib.term)
-  (q : query)
-  (domain_wf :
-    Forall (fun n => exists s, In (n, s) (declarations q)) (term_domain a))
-  : query :=
-  {|
-    assertions := a :: assertions q;
-    declarations := declarations q
-  |}.
-Next Obligation.
-  simpl.
-  rewrite lst_domain_cons.
-  rewrite List.Forall_app in *.
-  split.
-  - assumption.
-  - apply q.(wf).
-Qed.
+Definition add_assertion (a : term Sort_Bool) (q : query) : query := a :: q.
 
-Lemma add_assertion_reflect_if :
-  forall t q C P1 P2 domain_wf,
-    term_reflect_if C t P1 ->
-    smt_reflect_if C q P2 ->
-    smt_reflect_if C (add_assertion t q domain_wf) (fun ρ => P1 ρ /\ P2 ρ).
+Lemma add_assertion_reflect :
+  forall t q P1 P2,
+    term_reflect t P1 ->
+    smt_reflect q P2 ->
+    smt_reflect (add_assertion t q) (fun ρ => P1 ρ /\ P2 ρ).
 Proof.
-  destruct q.
-  unfold smt_reflect, smt_reflect_if, term_reflect, satisfied_by, combine.
+  unfold smt_reflect, term_reflect, satisfied_by, combine.
   simpl.
   intros.
   setoid_rewrite List.Forall_cons_iff.
   firstorder.
 Qed.
 
-Lemma add_assertion_reflect :
-  forall t q P1 P2 domain_wf,
-    term_reflect t P1 ->
-    smt_reflect q P2 ->
-    smt_reflect (add_assertion t q domain_wf) (fun ρ => P1 ρ /\ P2 ρ).
-Proof. intros. apply add_assertion_reflect_if; eassumption. Qed.
-
 Lemma unsat_smt_reflect_false q :
   unsatisfiable q <-> smt_reflect q (fun _ => False).
 Proof.
-  unfold smt_reflect, satisfied_by, combine.
-  simpl.
-  intros.
-  firstorder.
+  unfold smt_reflect, satisfied_by, combine, unsatisfiable, "⊧".
+  intuition eauto; expect 1.
+  rewrite <- H. eassumption.
 Qed.
 
-Lemma smt_reflect_if_rewrite : forall C P2 P1 q,
-    (forall ρ, C ρ -> P1 ρ <-> P2 ρ) ->
-    (smt_reflect_if C q P1 <-> smt_reflect_if C q P2).
+Lemma smt_reflect_rewrite : forall P2 P1 q,
+    (forall ρ, P1 ρ <-> P2 ρ) ->
+    (smt_reflect q P1 <-> smt_reflect q P2).
 Proof.
-  unfold smt_reflect, smt_reflect_if.
+  unfold smt_reflect.
   intros * HP.
   split; intros.
   - rewrite <- HP; eauto.
   - rewrite HP; eauto.
 Qed.
 
-Lemma smt_reflect_rewrite : forall P2 P1 q,
-    (forall ρ, P1 ρ <-> P2 ρ) ->
-    (smt_reflect q P1 <-> smt_reflect q P2).
-Proof. intros. eapply smt_reflect_if_rewrite. eauto. Qed.
-
 Lemma unsat_negation q P :
   smt_reflect q P ->
   unsatisfiable q ->
   (forall ρ, ~ P ρ).
 Proof.
-  unfold smt_reflect, smt_reflect_if, unsatisfiable.
+  unfold smt_reflect, unsatisfiable.
   intros Hreflect Hunsat * contra.
   repeat match goal with
          | [ H : forall (_ : valuation), _ |- _ ] => specialize (H ρ)
