vera/VerilogEquivalenceCorrectness.v
@@ -60,15 +60,15 @@ Ltac decompose_all_records :=
          | [ H : _ |- _ ] => progress (decompose record H); clear H
 	 end.
 
-Definition smt_same_value var (m : VerilogSMTBijection.t) (ρ : SMTQueries.valuation) :=
-  exists smtName1 smtName2 v,
+Definition smt_same_value var (m : VerilogSMTBijection.t) (ρ : SMTLib.valuation) :=
+  exists smtName1 smtName2,
     m (TaggedVariable.VerilogLeft, var) = Some smtName1 /\
       m (TaggedVariable.VerilogRight, var) = Some smtName2 /\
-      ρ smtName1 = Some v /\
-      ρ smtName2 = Some v.
+      ρ (SMTLib.Sort_BitVec (Verilog.varType var)) smtName1 =
+        ρ (SMTLib.Sort_BitVec (Verilog.varType var)) smtName2.
 
 Definition smt_all_same_values
-  (vars : list Verilog.variable) (m : VerilogSMTBijection.t) (ρ : SMTQueries.valuation) :=
+  (vars : list Verilog.variable) (m : VerilogSMTBijection.t) (ρ : SMTLib.valuation) :=
   Forall (fun verilogName => smt_same_value verilogName m ρ) vars.
 
 Lemma smt_all_same_values_cons var vars m ρ :
@@ -76,43 +76,29 @@ Lemma smt_all_same_values_cons var vars m ρ :
     smt_same_value var m ρ /\ smt_all_same_values vars m ρ.
 Proof. apply List.Forall_cons_iff. Qed.
 
-Definition smt_has_value tag (m : VerilogSMTBijection.t) var (ρ : SMTQueries.valuation) :=
-  exists smtName v, m (tag, var) = Some smtName /\ ρ smtName = Some v.
-
-Definition smt_all_have_values
-  tag vars (m : VerilogSMTBijection.t) (ρ : SMTQueries.valuation) :=
-  Forall (fun var => smt_has_value tag m var ρ) vars.
-
-Lemma smt_all_have_values_cons tag var vars m ρ :
-  smt_all_have_values tag (var :: vars) m ρ <->
-    smt_has_value tag m var ρ /\ smt_all_have_values tag vars m ρ.
-Proof. apply List.Forall_cons_iff. Qed.
-
-Definition smt_distinct_value (var : Verilog.variable) (m : VerilogSMTBijection.t) (ρ : SMTQueries.valuation) :=
-  exists smtName1 smtName2 v1 v2,
+Definition smt_distinct_value (var : Verilog.variable) (m : VerilogSMTBijection.t) (ρ : SMTLib.valuation) :=
+  exists smtName1 smtName2,
     m (TaggedVariable.VerilogLeft, var) = Some smtName1 /\
       m (TaggedVariable.VerilogRight, var) = Some smtName2 /\
-      ρ smtName1 = Some v1 /\
-      ρ smtName2 = Some v2 /\
-      v1 <> v2.
+      ρ (SMTLib.Sort_BitVec (Verilog.varType var)) smtName1 <>
+        ρ (SMTLib.Sort_BitVec (Verilog.varType var)) smtName2.
 
 Definition smt_some_distinct_values
-  vars (m : VerilogSMTBijection.t) (ρ : SMTQueries.valuation) :=
+  vars (m : VerilogSMTBijection.t) (ρ : SMTLib.valuation) :=
   Exists (fun verilogName => smt_distinct_value verilogName m ρ) vars.
 
 Definition counterexample_valuation v1 v2 m ρ :=
-  valid_execution v1 (SMT.execution_of_valuation TaggedVariable.VerilogLeft m ρ)
-  /\ valid_execution v2 (SMT.execution_of_valuation TaggedVariable.VerilogRight m ρ)
-  /\ smt_all_same_values (Verilog.module_inputs v1) m ρ
+  smt_all_same_values (Verilog.module_inputs v1) m ρ
   /\ smt_some_distinct_values (Verilog.module_outputs v1) m ρ
-  /\ smt_all_have_values TaggedVariable.VerilogLeft (Verilog.module_outputs v1) m ρ
-  /\ smt_all_have_values TaggedVariable.VerilogRight (Verilog.module_outputs v1) m ρ.
+  /\ valid_execution v1 (SMT.execution_of_valuation TaggedVariable.VerilogLeft m ρ)
+  /\ valid_execution v2 (SMT.execution_of_valuation TaggedVariable.VerilogRight m ρ)
+  .
 
 Definition execution_some_distinct_value (C : Verilog.variable -> Prop) (e1 e2 : execution) : Prop :=
   exists var bv1 bv2,
     C var
-    /\ e1 var = Some (XBV.from_bv bv1)
-    /\ e2 var = Some (XBV.from_bv bv2)
+    /\ e1 var = XBV.from_bv bv1
+    /\ e2 var = XBV.from_bv bv2
     /\ bv1 <> bv2.
 
 Definition counterexample_execution v1 e1 v2 e2 :=
@@ -126,10 +112,10 @@ Lemma smt_some_distinct_values_cons var vars m ρ :
     smt_distinct_value var m ρ \/ smt_some_distinct_values vars m ρ.
 Proof. apply List.Exists_cons. Qed.
 
-Lemma term_reflect_false C P :
-  (forall ρ, C ρ -> ~ P ρ) ->
-  term_reflect_if C SMTLib.Term_False P.
-Proof. unfold term_reflect_if, term_satisfied_by. crush. Qed.
+Lemma term_reflect_false P :
+  (forall ρ, ~ P ρ) ->
+  term_reflect SMTLib.Term_False P.
+Proof. unfold term_reflect, term_satisfied_by. crush. Qed.
 
 Lemma mk_var_same_spec : forall name m q,
   mk_var_same name m = inr q ->
@@ -138,23 +124,21 @@ Proof.
   intros * Hfunc.
   funelim (mk_var_same name m); try congruence.
   rewrite <- Heqcall in *. clear Heqcall. inv Hfunc.
-  intros ρ _.
+  intros ρ.
+  unfold smt_same_value, SMTQueries.term_satisfied_by.
+  simpl.
+  rewrite BV.bv_eq_reflect.
   split; intros * H.
-  - inv H. autodestruct_eqn E.
-    unfold smt_same_value.
-    rewrite SMTLib.value_eqb_eq in *. subst.
-    eauto 7.
-  - unfold SMTQueries.term_satisfied_by. simpl.
-    destruct H as [smt_name1' [smt_name2' [w [v [H0 [H1 H2]]]]]].
+  - eauto.
+  - destruct H as [smt_name1' [smt_name2' [H0 [H1 H2]]]].
     replace smt_name1' with smt_name1 in * by congruence.
     replace smt_name2' with smt_name2 in * by congruence.
-    rewrite H1, H2, SMTLib.value_eqb_refl.
-    reflexivity.
+    apply H2.
 Qed.
 
 Global Instance term_reflect_proper :
   Proper
-    (eq ==> pointwise_relation valuation iff ==> iff)
+    (eq ==> pointwise_relation SMTLib.valuation iff ==> iff)
     term_reflect.
 Proof.
   unfold term_reflect.
@@ -179,18 +163,6 @@ Proof.
     + apply IHinputs. assumption.
 Qed.
 
-(* TODO: Move me to smtcoqapi *)
-Lemma value_eqb_neq v1 v2 : SMTLib.value_eqb v1 v2 = false <-> v1 <> v2.
-Proof.
-  split; intros H.
-  - intros contra.
-    apply SMTLib.value_eqb_eq in contra.
-    congruence.
-  - destruct (SMTLib.value_eqb v1 v2) eqn:E; try reflexivity.
-    apply SMTLib.value_eqb_eq in E.
-    contradiction.
-Qed.
-
 Lemma mk_var_distinct_spec name m t :
   mk_var_distinct name m = inr t ->
   term_reflect t (smt_distinct_value name m).
@@ -198,79 +170,26 @@ Proof.
   intros * Hfunc.
   funelim (mk_var_distinct name m); try congruence.
   rewrite <- Heqcall in *. clear Heqcall. inv Hfunc.
-  intros ρ _.
+  intros ρ.
+  unfold term_satisfied_by, smt_distinct_value. simpl.
+  rewrite Bool.negb_true_iff.
+  rewrite BV.bv_neq_reflect.
   split; intros * H.
-  - inv H. autodestruct_eqn E.
-    rewrite Bool.negb_true_iff in *.
-    apply_somewhere value_eqb_neq. subst.
-    unfold smt_distinct_value.
-    eauto 10.
-  - unfold SMTQueries.term_satisfied_by. simpl.
-    destruct H as [smt_name1' [smt_name2' [w [v [v0 [H0 [H1 [H2 H3]]]]]]]].
+  - eauto.
+  - destruct H as [smt_name1' [smt_name2' [H0 [H1 H2]]]].
     replace smt_name1' with smt_name1 in * by congruence.
     replace smt_name2' with smt_name2 in * by congruence.
-    rewrite H1, H2.
-    apply value_eqb_neq in H3. rewrite H3.
-    reflexivity.
-Qed.
-
-Lemma term_reflect_if_cond_impl C1 C2 t P :
-  (forall ρ, C2 ρ -> C1 ρ) ->
-  term_reflect_if C1 t P ->
-  term_reflect_if C2 t P.
-Proof. unfold term_reflect_if. crush. Qed.
-
-Lemma mk_var_distinct_eval_spec var m ρ t :
-  mk_var_distinct var m = inr t ->
-  smt_has_value TaggedVariable.VerilogLeft m var ρ ->
-  smt_has_value TaggedVariable.VerilogRight m var ρ ->
-  exists b, SMTLib.interp_term ρ t = Some (SMTLib.Value_Bool b).
-Proof.
-  intros Hfunc Hhas_value_left Hhas_value_right.
-  funelim (mk_var_distinct var m); try congruence.
-  rewrite <- Heqcall in *. clear Heqcall. inv Hfunc.
-  destruct Hhas_value_left as [smtName_l [v_l [Hmatch_l Hv_l]]].
-  destruct Hhas_value_right as [smtName_r [v_r [Hmatch_r Hv_r]]].
-  replace smt_name1 with smtName_l in * by congruence.
-  replace smt_name2 with smtName_r in * by congruence.
-  simpl.
-  replace (ρ smtName_l). replace (ρ smtName_r).
-  eauto.
-Qed.
-
-Lemma mk_outputs_distinct_eval_spec outputs m ρ t :
-  mk_outputs_distinct outputs m = inr t ->
-  smt_all_have_values TaggedVariable.VerilogLeft outputs m ρ ->
-  smt_all_have_values TaggedVariable.VerilogRight outputs m ρ ->
-  exists b, SMTLib.interp_term ρ t = Some (SMTLib.Value_Bool b).
-Proof.
-  revert t.
-  induction outputs; simp mk_outputs_distinct;
-    intros t Hfunc Hhave_values_left Hhave_values_right.
-  - inv Hfunc. simpl. eauto.
-  - autodestruct_eqn E.
-    rewrite smt_all_have_values_cons in Hhave_values_left, Hhave_values_right.
-    destruct Hhave_values_left as [Hhas_value_left Hhave_values_left].
-    destruct Hhave_values_right as [Hhas_value_right Hhave_values_right].
-    edestruct mk_var_distinct_eval_spec as [b1 Hb1]; eauto.
-    edestruct IHoutputs as [b2 Hb2]; eauto.
-    simpl. rewrite Hb1, Hb2.
-    eauto.
+    apply H2.
 Qed.
 
 Lemma mk_outputs_distinct_spec outputs m t :
   mk_outputs_distinct outputs m = inr t ->
-  term_reflect_if
-    (fun ρ =>
-       smt_all_have_values TaggedVariable.VerilogLeft outputs m ρ
-       /\ smt_all_have_values TaggedVariable.VerilogRight outputs m ρ)
-    t
-    (smt_some_distinct_values outputs m).
+  term_reflect t (smt_some_distinct_values outputs m).
 Proof.
   revert t m. induction outputs.
   - intros * H. simp mk_outputs_distinct in H. inv H.
     apply term_reflect_false.
-    intros ρ _ contra.
+    intros ρ contra.
     inv contra.
   - intros.
     simp mk_outputs_distinct in H.
@@ -278,18 +197,10 @@ Proof.
     insterU IHoutputs.
     unfold smt_some_distinct_values.
     setoid_rewrite List.Exists_cons.
-    eapply term_reflect_if_cond_impl; cycle 1. {
-      eapply term_reflect_or.
-      - apply mk_var_distinct_spec.
-        eassumption.
-      - eapply IHoutputs.
-    }
-    simpl.
-    setoid_rewrite smt_all_have_values_cons.
-    intros ρ [[Hvals1 Hvals2] [Hvals3 Hvals4]].
-    (intuition try assumption); [|].
-    + eapply mk_var_distinct_eval_spec; eauto.
-    + eapply mk_outputs_distinct_eval_spec; eauto.
+    apply term_reflect_or.
+    + apply mk_var_distinct_spec.
+      eassumption.
+    + eapply IHoutputs.
 Qed.
 
 Lemma execution_of_valuation_map_equal (m1 m2 : VerilogSMTBijection.t) tag ρ:
@@ -304,58 +215,39 @@ Proof.
   reflexivity.
 Qed.
 
-Lemma verilog_to_smt_outputs_have_values tag start v s ρ:
-  VerilogToSMT.verilog_to_smt tag start v = inr s ->
-  ρ ⊧ SMT.query s ->
-  smt_all_have_values tag (Verilog.module_outputs v) (SMT.nameMap s) ρ.
-Proof.
-  unfold VerilogToSMT.verilog_to_smt, smt_all_have_values, smt_has_value, "⊧", valuation_matches_decls.
-  intros H.
-  monad_inv. simpl in *. intros [Hdecls Hassertions].
-  intros.
-  rewrite List.Forall_forall. intros var Hvar_in.
-  apply Verilog.module_outputs_in_vars in Hvar_in.
-  pose proof VerilogToSMTCorrect.declarations_satisfied_valuation_has_var as H.
-  insterU H. destruct H as [smtName [bv [Ht Hρ]]].
-  eauto.
-Qed.
-
-Lemma satisfied_by_add_assertion_iff t q prf ρ :
-  satisfied_by ρ (add_assertion t q prf) <->
+Lemma satisfied_by_cons_iff t q ρ :
+  satisfied_by ρ (t :: q) <->
   term_satisfied_by ρ t /\ satisfied_by ρ q.
-Proof.
-  unfold add_assertion, satisfied_by.
-  simpl.
-  rewrite List.Forall_cons_iff.
-  crush.
-Qed.
+Proof. apply List.Forall_cons_iff. Qed.
 
-Lemma satisfied_by_combine_iff q1 q2 ρ :
-  satisfied_by ρ (SMTQueries.combine q1 q2) <->
+Lemma satisfied_by_app_iff q1 q2 ρ :
+  satisfied_by ρ (q1 ++ q2)%list <->
   satisfied_by ρ q1 /\ satisfied_by ρ q2.
-Proof.
-  unfold SMTQueries.combine, satisfied_by, valuation_matches_decls.
-  simpl.
-  rewrite ! List.Forall_app.
-  crush.
-Qed.
+Proof. apply List.Forall_app. Qed.
 
-Lemma smt_has_value_tag_equal (m1 m2 : VerilogSMTBijection.t) var tag ρ :
-  (forall var, m1 (tag, var) = m2 (tag, var)) ->
-  smt_has_value tag m1 var ρ <-> smt_has_value tag m2 var ρ.
+Lemma smt_reflect_cons t q P1 P2 :
+  term_reflect t P1 ->
+  smt_reflect q P2 ->
+  smt_reflect (t :: q) (fun ρ => P1 ρ /\ P2 ρ).
 Proof.
-  unfold smt_has_value.
-  intros H. rewrite H. reflexivity.
+  unfold term_reflect, smt_reflect.
+  intros H1 H2.
+  setoid_rewrite satisfied_by_cons_iff.
+  setoid_rewrite H1.
+  setoid_rewrite H2.
+  reflexivity.
 Qed.
-
-Lemma smt_all_have_values_tag_equal (m1 m2 : VerilogSMTBijection.t) vars tag ρ :
-  (forall var, m1 (tag, var) = m2 (tag, var)) ->
-  smt_all_have_values tag vars m1 ρ <-> smt_all_have_values tag vars m2 ρ.
+  
+Lemma smt_reflect_app q1 q2 P1 P2 :
+  smt_reflect q1 P1 ->
+  smt_reflect q2 P2 ->
+  smt_reflect (q1 ++ q2)%list (fun ρ => P1 ρ /\ P2 ρ).
 Proof.
-  unfold smt_all_have_values.
-  rewrite ! List.Forall_forall.
-  intros.
-  setoid_rewrite smt_has_value_tag_equal; eauto.
+  unfold term_reflect, smt_reflect.
+  intros H1 H2.
+  setoid_rewrite satisfied_by_app_iff.
+  setoid_rewrite H1.
+  setoid_rewrite H2.
   reflexivity.
 Qed.
 
@@ -372,78 +264,27 @@ Proof.
   remember (VerilogSMTBijection.combine _ _ _ _) as m_combined.
   unfold counterexample_valuation.
 
-  eapply smt_reflect_if_elim.
-  - eapply smt_reflect_if_rewrite; cycle 1.
-    + apply add_assertion_reflect_if. {
-        apply mk_outputs_distinct_spec; eassumption.
-      }
-      apply add_assertion_reflect_if. {
-        apply term_reflect_if_intro.
-        apply mk_inputs_same_spec; eassumption.
-      }
-      apply smt_reflect_if_intro.
-      apply concat_conj.
-      * eapply VerilogToSMTCorrect.verilog_to_smt_correct.
-        eassumption.
-      * eapply VerilogToSMTCorrect.verilog_to_smt_correct.
-        eassumption.
-    + simpl. intros ρ [Hvalues_left Hvalues_right].
-      split; intros H; decompose record H; clear H;
-        unpack_goal; try eassumption.
-      * erewrite execution_of_valuation_map_equal; [eassumption|].
-        replace m_combined. intros. symmetry.
-        eapply VerilogSMTBijection.combine_different_tag_left
-          with (t2 := TaggedVariable.VerilogRight).
-        -- discriminate.
-        -- eapply verilog_to_smt_only_tag; eassumption.
-        -- eapply verilog_to_smt_only_tag; eassumption.
-      * erewrite execution_of_valuation_map_equal; [eassumption|].
-        replace m_combined. intros. symmetry.
-        eapply VerilogSMTBijection.combine_different_tag_right
-          with (t1 := TaggedVariable.VerilogLeft).
-        -- discriminate.
-        -- eapply verilog_to_smt_only_tag; eassumption.
-        -- eapply verilog_to_smt_only_tag; eassumption.
-      * erewrite execution_of_valuation_map_equal; [eassumption|].
-        replace m_combined. intros.
-        eapply VerilogSMTBijection.combine_different_tag_left
-          with (t2 := TaggedVariable.VerilogRight).
-        -- discriminate.
-        -- eapply verilog_to_smt_only_tag; eassumption.
-        -- eapply verilog_to_smt_only_tag; eassumption.
-      * erewrite execution_of_valuation_map_equal; [eassumption|].
-        replace m_combined. intros.
-        eapply VerilogSMTBijection.combine_different_tag_right
-          with (t1 := TaggedVariable.VerilogLeft).
-        -- discriminate.
-        -- eapply verilog_to_smt_only_tag; eassumption.
-        -- eapply verilog_to_smt_only_tag; eassumption.
-  - simpl. intros. crush.
-  - simpl.
-    intros ρ H.
-    rewrite ! satisfied_by_add_assertion_iff, satisfied_by_combine_iff in H.
-    decompose record H. clear H.
-    replace m_combined.
-    split.
-    + eapply smt_all_have_values_tag_equal. {
-        intros.
-        eapply VerilogSMTBijection.combine_different_tag_left
-          with (t2 := TaggedVariable.VerilogRight).
-        - discriminate.
-        - eapply verilog_to_smt_only_tag; eassumption.
-        - eapply verilog_to_smt_only_tag; eassumption.
-      }
-      eapply verilog_to_smt_outputs_have_values; eassumption.
-    + eapply smt_all_have_values_tag_equal. {
-        intros.
-        eapply VerilogSMTBijection.combine_different_tag_right
-          with (t1 := TaggedVariable.VerilogLeft).
-        - discriminate.
-        - eapply verilog_to_smt_only_tag; eassumption.
-        - eapply verilog_to_smt_only_tag; eassumption.
-      }
-      replace (Verilog.module_outputs verilog1).
-      eapply verilog_to_smt_outputs_have_values; try eassumption.
+  repeat (apply smt_reflect_cons || apply smt_reflect_app); expect 4.
+  - apply mk_inputs_same_spec; eassumption.
+  - apply mk_outputs_distinct_spec; eassumption.
+  - setoid_rewrite execution_of_valuation_map_equal. 
+    + eapply VerilogToSMTCorrect.verilog_to_smt_correct.
+      eassumption.
+    + replace m_combined. intros.
+      eapply VerilogSMTBijection.combine_different_tag_left
+        with (t2 := TaggedVariable.VerilogRight).
+      * discriminate.
+      * eapply verilog_to_smt_only_tag; eassumption.
+      * eapply verilog_to_smt_only_tag; eassumption.
+  - setoid_rewrite execution_of_valuation_map_equal. 
+    + eapply VerilogToSMTCorrect.verilog_to_smt_correct.
+      eassumption.
+    + replace m_combined. intros.
+      eapply VerilogSMTBijection.combine_different_tag_right
+        with (t1 := TaggedVariable.VerilogLeft).
+      * discriminate.
+      * eapply verilog_to_smt_only_tag; eassumption.
+      * eapply verilog_to_smt_only_tag; eassumption.
 Qed.
 
 Lemma smt_same_values_eq var vars m n1 n2 ρ :
@@ -451,110 +292,81 @@ Lemma smt_same_values_eq var vars m n1 n2 ρ :
   In var vars ->
   m (TaggedVariable.VerilogLeft, var) = Some n1 ->
   m (TaggedVariable.VerilogRight, var) = Some n2 ->
-  ρ n1 = ρ n2.
+  ρ (SMTLib.Sort_BitVec (Verilog.varType var)) n1 = ρ (SMTLib.Sort_BitVec (Verilog.varType var)) n2.
 Proof.
   unfold smt_all_same_values, smt_same_value.
   intros Hmatch Hin Hm1 Hm2.
   rewrite List.Forall_forall in Hmatch.
   insterU Hmatch.
-  destruct Hmatch as [n1' [n2'[v [? [? [? ?]]]]]].
+  destruct Hmatch as [n1' [n2' [? [? ?]]]].
   replace n1' with n1 in * by crush.
   replace n2' with n2 in * by crush.
   crush.
 Qed.
 
-Lemma execution_of_valuation_inv tag m ρ var bv :
-  SMT.execution_of_valuation tag m ρ var = Some (XBV.from_bv bv) ->
-  exists smtName,
-    m (tag, var) = Some smtName /\
-    ρ smtName = Some (SMTLib.Value_BitVec (Verilog.varType var) bv).
-Proof.
-  unfold SMT.execution_of_valuation.
-  intros H.
-  autodestruct_eqn E. simpl in *.
-  apply XBV.from_bv_injective in H1; subst.
-  eauto.
-Qed.
-
-Lemma valid_execution_of_valuation_match v tag m ρ :
-  Permutation (Verilog.module_body_writes (Verilog.modBody v)) (Verilog.module_outputs v) ->
-  VerilogToSMT.all_vars_driven v ->
-  valid_execution v (SMT.execution_of_valuation tag m ρ) ->
-  verilog_smt_match_states_partial
-    (fun var => In var (Verilog.modVariables v))
-    tag m (SMT.execution_of_valuation tag m ρ) ρ.
-Proof.
-  unfold verilog_smt_match_states_partial.
-  intros Houtputs Hdriven Hvalid.
-  apply VerilogToSMTCorrect.valid_execution_complete in Hvalid; [|assumption|eassumption].
-  unfold complete_execution, RegisterState.has_value_for in Hvalid.
-  intros var Hvar_in. insterU Hvalid.
-  destruct Hvalid as [xbv Hxbv].
-  pose proof SMT.execution_of_valuation_no_exes as H.
-  insterU H. rewrite XBV.not_has_x_to_bv in H.
-  destruct H as [bv Hbv]. apply XBV.bv_xbv_inverse in Hbv. subst xbv.
-  edestruct execution_of_valuation_inv as [smtName [Hm Hρ]]; [eassumption|].
-  eexists. split; [eassumption|].
-  econstructor; try eassumption; [].
-  constructor.
-Qed.
+(* Lemma valid_execution_of_valuation_match v tag m ρ :
+ *   Permutation (Verilog.module_body_writes (Verilog.modBody v)) (Verilog.module_outputs v) ->
+ *   VerilogToSMT.all_vars_driven v ->
+ *   valid_execution v (SMT.execution_of_valuation tag m ρ) ->
+ *   verilog_smt_match_states_partial
+ *     (fun var => In var (Verilog.modVariables v))
+ *     tag m (SMT.execution_of_valuation tag m ρ) ρ.
+ * Proof.
+ *   intros Houtputs Hdriven Hvalid.
+ *   pose proof (verilog_smt_match_states_execution_of_valuation_same tag m ρ).
+ * Admitted. *)
 
 Lemma smt_distinct_values_not_defined_match vars m ρ :
   smt_some_distinct_values vars m ρ ->
-  ~ (SMT.execution_of_valuation TaggedVariable.VerilogLeft m ρ =!!(
+  ~ (SMT.execution_of_valuation TaggedVariable.VerilogLeft m ρ =(
        vars
-     )!!= SMT.execution_of_valuation TaggedVariable.VerilogRight m ρ).
+     )= SMT.execution_of_valuation TaggedVariable.VerilogRight m ρ).
 Proof.
   unfold smt_some_distinct_values.
-  rewrite RegisterState.defined_match_on_iff, List.Exists_exists.
-  intros [var [Hin Hsmt_distinct]] Hcontra.
-  edestruct Hcontra as [bv [Hleft Hright]]; [eassumption|]. clear Hcontra.
-  apply execution_of_valuation_inv in Hleft.
-  apply execution_of_valuation_inv in Hright.
+  rewrite List.Exists_exists.
+  intros [var [Hin Hsmt_distinct]] contra.
   unfold smt_distinct_value in Hsmt_distinct.
-
-  decompose_all_records. crush.
+  unfold "_ =( _ )= _" in contra.
+  specialize (contra var Hin).
+  unfold SMT.execution_of_valuation in contra.
+  decompose_all_records. 
+  replace (m (TaggedVariable.VerilogLeft, var)) in contra.
+  replace (m (TaggedVariable.VerilogRight, var)) in contra.
+  apply XBV.from_bv_injective in contra.
+  contradiction.
 Qed.
 
-Lemma smt_all_same_inputs_execution_match v1 v2 m ρ :
-  Permutation (Verilog.module_body_writes (Verilog.modBody v1)) (Verilog.module_outputs v1) ->
-  Permutation (Verilog.module_body_writes (Verilog.modBody v2)) (Verilog.module_outputs v2) ->
-  VerilogToSMT.all_vars_driven v1 ->
-  VerilogToSMT.all_vars_driven v2 ->
-  valid_execution v1 (SMT.execution_of_valuation TaggedVariable.VerilogLeft m ρ) ->
-  valid_execution v2 (SMT.execution_of_valuation TaggedVariable.VerilogRight m ρ) ->
-  Verilog.module_inputs v1 = Verilog.module_inputs v2 ->
-  smt_all_same_values (Verilog.module_inputs v1) m ρ ->
+Lemma smt_all_same_values_execution_match vars m ρ :
+  smt_all_same_values vars m ρ ->
   (SMT.execution_of_valuation TaggedVariable.VerilogLeft m ρ) =!!(
-    Verilog.module_inputs v1
+    vars
   )!!= (SMT.execution_of_valuation TaggedVariable.VerilogRight m ρ).
 Proof.
-  unfold smt_all_same_values.
-  rewrite RegisterState.defined_match_on_iff.
-  intros Houtputs1 Houtputs2 Hdriven1 Hdriven2 Hvalid1 Hvalid2 Hmatch_inputs Hsmt_same var Hvar_in.
-  edestruct (valid_execution_of_valuation_match v1) as
-    [smtName_left [Hm_left [xbv_l val_l Hsmtval_l Hverilogval_l Hmatchvals_l]]];
-    [ assumption
-    | eassumption
-    | eassumption
-    | apply Verilog.module_input_in_vars; eassumption
-    |].
-  edestruct (valid_execution_of_valuation_match v2) as
-    [smtName_right [Hm_right [xbv_r val_r Hsmtval_r Hverilogval_r Hmatchvals_r]]];
-    [ assumption
-    | eassumption
-    | eassumption
-    | apply Verilog.module_input_in_vars; rewrite <- Hmatch_inputs; eassumption
-    |].
-  rewrite Hverilogval_l, Hverilogval_r.
-  replace val_r with val_l in *.
-  - inv Hmatchvals_l. inv Hmatchvals_r.
-    crush.
-  - pose proof smt_same_values_eq as Heq.
-    insterU Heq.
-    rewrite Hsmtval_l, Hsmtval_r in Heq.
-    inv Heq. reflexivity.
+  unfold smt_all_same_values, smt_same_value.
+  rewrite List.Forall_forall.
+  intros Hmatch.
+  apply RegisterState.defined_match_on_iff.
+  intros var Hvar. specialize (Hmatch var Hvar).
+  destruct Hmatch as [smtName1 [smtName2 [Hm1 [Hm2 Hmatch]]]].
+  unfold SMT.execution_of_valuation.
+  rewrite Hm1, Hm2, Hmatch. 
+  eauto.
 Qed.
+
+(* Replace me with above *)
+(* Lemma smt_all_same_inputs_execution_match v1 v2 m ρ :
+ *   Permutation (Verilog.module_body_writes (Verilog.modBody v1)) (Verilog.module_outputs v1) ->
+ *   Permutation (Verilog.module_body_writes (Verilog.modBody v2)) (Verilog.module_outputs v2) ->
+ *   VerilogToSMT.all_vars_driven v1 ->
+ *   VerilogToSMT.all_vars_driven v2 ->
+ *   valid_execution v1 (SMT.execution_of_valuation TaggedVariable.VerilogLeft m ρ) ->
+ *   valid_execution v2 (SMT.execution_of_valuation TaggedVariable.VerilogRight m ρ) ->
+ *   Verilog.module_inputs v1 = Verilog.module_inputs v2 ->
+ *   smt_all_same_values (Verilog.module_inputs v1) m ρ ->
+ *   (SMT.execution_of_valuation TaggedVariable.VerilogLeft m ρ) =!!(
+ *     Verilog.module_inputs v1
+ *   )!!= (SMT.execution_of_valuation TaggedVariable.VerilogRight m ρ).
+ * Admitted. *)
 
 Lemma execution_defined_match_smt_all_same_values vars m ρ :
   (SMT.execution_of_valuation TaggedVariable.VerilogLeft m ρ) =!!(
@@ -573,28 +385,7 @@ Proof.
 
   eapply execution_of_valuation_inv in Hlookup_right.
   decompose record Hlookup_right. clear Hlookup_right.
-  eauto 10.
-Qed.
-
-Lemma valid_execution_smt_all_outputs_have_values v tag m ρ :
-  Permutation (Verilog.module_body_writes (Verilog.modBody v)) (Verilog.module_outputs v) ->
-  VerilogToSMT.all_vars_driven v ->
-  valid_execution v (SMT.execution_of_valuation tag m ρ) ->
-  smt_all_have_values tag (Verilog.module_outputs v) m ρ.
-Proof.
-  intros Houtputs Hvars_driven Hvalid.
-  pose proof (VerilogToSMTCorrect.valid_execution_complete v) as H.
-  insterU H. clear Hvalid Hvars_driven.
-  unfold complete_execution, smt_all_have_values, smt_has_value in *.
-  apply List.Forall_forall. intros var Hvar_in.
-  apply Verilog.module_outputs_in_vars in Hvar_in.
-  edestruct H as [xbv Hlookup]; [eassumption|clear H].
-  pose proof SMT.execution_of_valuation_no_exes as H.
-  insterU H. rewrite XBV.not_has_x_to_bv in H.
-  destruct H as [bv Hbv]. apply XBV.bv_xbv_inverse in Hbv. subst xbv.
-  eapply execution_of_valuation_inv in Hlookup.
-  decompose record Hlookup. clear Hlookup.
-  eauto.
+  eexists. eexists. unpack_goal; crush.
 Qed.
 
 Lemma imply_or_iff P Q :
@@ -656,9 +447,8 @@ Proof.
   apply execution_of_valuation_inv in Hlookup_left. decompose record Hlookup_left.
   apply execution_of_valuation_inv in Hlookup_right. decompose record Hlookup_right.
   eexists. split; [eassumption|].
-  do 4 eexists. repeat split; eauto.
-  intro contra. inv contra.
-  contradiction.
+  do 2 eexists.
+  unpack_goal; crush.
 Qed.
 
 Lemma all_driven_outputs_driven v :
@@ -691,60 +481,15 @@ Proof.
 Qed.
 
 (* TODO: Move me to Match.v *)
-Lemma execution_of_valuation_all_defined C tag m ρ :
-  RegisterState.has_value_for C (SMT.execution_of_valuation tag m ρ) ->
-  RegisterState.defined_value_for C (SMT.execution_of_valuation tag m ρ).
+Lemma execution_of_valuation_all_defined tag (m : VerilogSMTBijection.t) ρ :
+  RegisterState.defined_value_for
+    (fun var => exists n, m (tag, var) = Some n)
+    (SMT.execution_of_valuation tag m ρ).
 Proof.
-  unfold RegisterState.has_value_for, RegisterState.defined_value_for.
-  intros * Hhas_value var HC.
-  insterU Hhas_value. destruct Hhas_value as [xbv Hlookup].
-  rewrite Hlookup.
-  unfold SMT.execution_of_valuation in Hlookup.
-  autodestruct_eqn E. crush.
+  unfold RegisterState.defined_value_for, SMT.execution_of_valuation.
+  intros var [n HC].
+  crush.
 Qed.
-
-Lemma valid_execution_has_value_for_writes v e :
-  Permutation (Verilog.module_body_writes (Verilog.modBody v)) (Verilog.module_outputs v) ->
-  valid_execution v e ->
-  RegisterState.has_value_for
-    (fun var : Verilog.variable => In var (Verilog.module_body_writes (Verilog.modBody v)))
-    e.
-Proof.
-  unfold valid_execution. intros Houtputs Hvalid. 
-  decompose record Hvalid. setoid_rewrite Houtputs. assumption.
-Qed.
-
-Lemma valid_execution_has_value_for_inputs v e :
-  valid_execution v e ->
-  RegisterState.has_value_for
-    (fun var : Verilog.variable => In var (Verilog.module_inputs v))
-    e.
-Proof.
-  unfold valid_execution. intros Hvalid. 
-  decompose record Hvalid. assumption.
-Qed.
-
-Lemma valuation_has_var_tag_equal tag (m1 m2 : VerilogSMTBijection.t) ρ var :
-  (forall n, m1 (tag, n) = m2 (tag, n)) ->
-  valuation_has_var tag m1 ρ var <-> valuation_has_var tag m2 ρ var.
-Proof.
-  unfold valuation_has_var.
-  intros Heq.
-  split.
-  all:
-    intros Hmatch;
-    decompose record Hmatch;
-    rewrite Heq in *;
-    eauto.
-Qed.
-
-Ltac inv_equivalence_query_sat :=
-  match goal with
-  | [ Hfunc: equivalence_query _ _ = inr ?smt, Hsat : _ ⊧ SMT.query ?smt |- _ ] =>
-      unfold equivalence_query in Hfunc; monad_inv; simpl in *;
-      rewrite ! satisfied_by_add_assertion_iff, satisfied_by_combine_iff in Hsat;
-      decompose record Hsat
-  end.
 
 Local Open Scope verilog.
 
@@ -761,20 +506,14 @@ Proof.
   unfold valid_execution.
   RegisterState.unpack_match_on.
   split.
-  - intros H1. decompose record H1. clear H1.
-    RegisterState.unpack_match_on.
-    setoid_rewrite H0 at 2 in H3.
-    rewrite H0 in *.
-    rewrite H in *.
-    unpack_goal; try eassumption; expect 1.
-    RegisterState.unpack_match_on; eassumption.
-  - intros H1. decompose record H1. clear H1.
-    RegisterState.unpack_match_on.
-    setoid_rewrite <- H0 at 2 in H3.
-    rewrite <- H0 in *.
-    rewrite <- H in *.
-    unpack_goal; try eassumption; expect 1.
-    RegisterState.unpack_match_on; eassumption.
+  all: intros H1.
+  - rewrite <- H at 1.
+    rewrite H1.
+    RegisterState.unpack_match_on; assumption.
+  - rewrite H at 1.
+    rewrite H1.
+    symmetry.
+    RegisterState.unpack_match_on; assumption.
 Qed.
 
 (* Lemma transfer_execution v e :
@@ -807,15 +546,13 @@ Lemma clean_defined_outputs v e :
   RegisterState.defined_value_for
     (fun var : Verilog.variable => In var (Verilog.module_outputs v)) e.
 Proof.
-  unfold clean_module, "⇓".
-  intros Hclean [Hinputs_e [Houtputs_e Hmatch]] Hinputs. 
-  specialize (Hclean e). insterU Hclean.
-  destruct Hclean as [Hmatch_inputs Hdefined_outputs].
-  (* replace e'' with e' in * by congruence. *)
+  unfold "⇓".
+  intros Hclean Hmatch Hinputs. 
   RegisterState.unpack_match_on.
-  rename_match (_ =( Verilog.module_outputs v )= e) into Hmatch_outputs.
+  rename_match (_ =( Verilog.module_outputs _ )= _) into Hmatch_outputs.
   rewrite <- Hmatch_outputs.
-  assumption.
+  apply Hclean.
+  apply Hinputs.
 Qed.
 
 Ltac assert_rewrite r :=
@@ -872,28 +609,14 @@ Lemma execution_congruent v e1 e2 :
 Proof.
   unfold "⇓".
   intros Hadmit1 Hadmit2 Hinput_match.
-  decompose record Hadmit1. clear Hadmit1.
-  decompose record Hadmit2. clear Hadmit2.
   RegisterState.unpack_match_on.
-  rename_match (run_vmodule v (e1 // _) =( Verilog.module_outputs _ )= e1) into Houtputs1.
+  rename_match (run_vmodule v e1 =( Verilog.module_outputs _ )= e1) into Houtputs1.
   rewrite <- Houtputs1.
-  rename_match (run_vmodule v (e2 // _) =( Verilog.module_outputs _ )= e2) into Houtputs2.
+  rename_match (run_vmodule v e2 =( Verilog.module_outputs _ )= e2) into Houtputs2.
   rewrite <- Houtputs2.
   rewrite Hinput_match.
   reflexivity.
 Qed.
-
-Lemma admit_run_vmodule v e:
-  RegisterState.has_value_for (fun var => In var (Verilog.module_inputs v)) e ->
-  v ⇓ (run_vmodule v (e // Verilog.module_inputs v)).
-Proof.
-  intros Hhas_inputs.
-  unfold "⇓".
-  unpack_goal.
-  - admit. (* has inputs *)
-  - admit. (* has outputs *)
-  - admit. (* preserve inputs *)
-Admitted.
 
 Lemma no_counterexample_equivalent_iff v1 v2 :
   Verilog.module_inputs v1 = Verilog.module_inputs v2 ->
@@ -911,28 +634,24 @@ Proof.
     split; intros He.
     (* This is duplicated, ideally we want a "without loss of generality" tactic *)
     + RegisterState.unpack_defined_value_for.
-      assert (Hrun2 : v2 ⇓ run_vmodule v2 (e // Verilog.module_inputs v2)). {
-        apply admit_run_vmodule. 
-	apply VerilogToSMTCorrect.defined_value_for_has_value_for.
-	rewrite <- Hinput_match.
-	assumption.
+      assert (Hrun2 : v2 ⇓ run_vmodule v2 e). {
+        apply admit_run_vmodule.
+	apply Hclean2.
       }
-      assert (Hmatch_inputs : e =!!( Verilog.module_inputs v1 )!!= run_vmodule v2 (e // Verilog.module_inputs v2)). {
+      assert (Hmatch_inputs : e =!!( Verilog.module_inputs v1 )!!= run_vmodule v2 e). {
 	split; [|assumption].
-	edestruct Hclean2.
-	- rewrite <- Hinput_match.
-	  eassumption.
-	- rewrite Hinput_match.
-	  eassumption.
+	symmetry.
+	rewrite Hinput_match.
+	apply Hclean2.
       }
-      specialize (H e (run_vmodule v2 (e // Verilog.module_inputs v2))).
+      specialize (H e (run_vmodule v2 e)).
       apply not_and_or in H. destruct H; [contradiction|].
       apply not_and_or in H. destruct H; [contradiction|].
       apply not_and_or in H. destruct H; [contradiction|].
       apply NNPP in H.
       assert (Hmatch_all :
         e =( Verilog.module_inputs v2 ++ Verilog.module_outputs v2
-	  )= run_vmodule v2 (e // Verilog.module_inputs v2)). {
+	  )= run_vmodule v2 e). {
 	  RegisterState.unpack_match_on.
 	- rewrite Hinput_match in Hmatch_inputs.
 	  destruct Hmatch_inputs. assumption.
@@ -941,19 +660,16 @@ Proof.
       rewrite Hmatch_all.
       assumption.
     + RegisterState.unpack_defined_value_for.
-      assert (Hrun1 : v1 ⇓ run_vmodule v1 (e // Verilog.module_inputs v1)). {
-        apply admit_run_vmodule. 
-	apply VerilogToSMTCorrect.defined_value_for_has_value_for.
-	assumption.
+      assert (Hrun1 : v1 ⇓ run_vmodule v1 e). {
+        apply admit_run_vmodule.
+	apply Hclean1.
       }
-      assert (Hmatch_inputs : e =!!( Verilog.module_inputs v1 )!!= run_vmodule v1 (e // Verilog.module_inputs v1)). {
+      assert (Hmatch_inputs : e =!!( Verilog.module_inputs v1 )!!= run_vmodule v1 e). {
 	split; [|assumption].
-	unfold clean_module in Hclean1.
-	edestruct Hclean1.
-	- eassumption.
-	- eassumption.
+	symmetry.
+	apply Hclean1.
       }
-      specialize (H (run_vmodule v1 (e // Verilog.module_inputs v1)) e).
+      specialize (H (run_vmodule v1 e) e).
       apply not_and_or in H. destruct H; [contradiction|].
       apply not_and_or in H. destruct H; [contradiction|].
       apply not_and_or in H. destruct H; [symmetry in Hmatch_inputs; contradiction|].
@@ -961,7 +677,7 @@ Proof.
       assert_rewrite (
           e =(
 	    Verilog.module_inputs v1 ++ Verilog.module_outputs v1
-          )= run_vmodule v1 (e // Verilog.module_inputs v1)). {
+          )= run_vmodule v1 e). {
 	RegisterState.unpack_match_on.
 	- destruct Hmatch_inputs. assumption.
 	- symmetry. assumption.
@@ -1080,12 +796,12 @@ Proof.
   constructor; eauto using verilog_to_smt_checks.
 Qed.
 
-Lemma counterexample_valuation_execution v1 v2 m ρ q :
+Lemma counterexample_valuation_execution v1 v2 ρ q :
   equivalence_query_checked v1 v2 q ->
-  counterexample_valuation v1 v2 m ρ <->
+  counterexample_valuation v1 v2 (SMT.nameMap q) ρ <->
     counterexample_execution
-      v1 (SMT.execution_of_valuation TaggedVariable.VerilogLeft m ρ)
-      v2 (SMT.execution_of_valuation TaggedVariable.VerilogRight m ρ).
+      v1 (SMT.execution_of_valuation TaggedVariable.VerilogLeft (SMT.nameMap q) ρ)
+      v2 (SMT.execution_of_valuation TaggedVariable.VerilogRight (SMT.nameMap q) ρ).
 Proof.
   intros Hequivalence_query.
   destruct Hequivalence_query.
@@ -1096,34 +812,26 @@ Proof.
   - unpack_goal.
     + assumption.
     + assumption.
-    + eapply smt_all_same_inputs_execution_match;
-        eassumption.
-    + rename_match (smt_some_distinct_values (Verilog.module_outputs v1) m ρ)
-        into Houtputs_distinct_smt.
-      apply smt_distinct_values_not_defined_match in Houtputs_distinct_smt.
-      intro contra. apply Houtputs_distinct_smt. clear Houtputs_distinct_smt.
-      split; [assumption|].
-      setoid_rewrite all_driven_outputs_driven; try assumption; expect 1.
-      apply execution_of_valuation_all_defined.
-      apply valid_execution_has_value_for_writes; assumption.
+    + apply smt_all_same_values_execution_match. assumption.
+    + apply smt_distinct_values_not_defined_match. assumption.
   - unpack_goal.
-    + eassumption.
-    + eassumption.
-    + apply execution_defined_match_smt_all_same_values.
-      assumption.
+    + apply execution_defined_match_smt_all_same_values. assumption.
     + apply not_execution_defined_match_on_smt_some_distinct_values; expect 1.
       apply not_defined_match_some_distinct.
-      * setoid_rewrite all_driven_outputs_driven; try assumption; expect 1.
-	apply execution_of_valuation_all_defined.
-        apply valid_execution_has_value_for_writes; assumption.
-      * rewrite inputs_match0, outputs_match0 in *.
-        setoid_rewrite all_driven_outputs_driven; try assumption; expect 1.
-	apply execution_of_valuation_all_defined.
-        apply valid_execution_has_value_for_writes; assumption.
+      * eapply RegisterState.defined_value_for_impl; [|apply execution_of_valuation_all_defined].
+	simpl. intros.
+	apply map_match_left0.
+	apply Verilog.module_outputs_in_vars.
+	assumption.
+      * eapply RegisterState.defined_value_for_impl; [|apply execution_of_valuation_all_defined].
+	simpl. intros.
+	apply map_match_right0.
+	apply Verilog.module_outputs_in_vars.
+	rewrite <- outputs_match0.
+	assumption.
       * unfold "_ =!!( _ )!!= _". intuition eauto.
-    + eapply valid_execution_smt_all_outputs_have_values; eassumption.
-    + rewrite inputs_match0, outputs_match0 in *.
-      eapply valid_execution_smt_all_outputs_have_values; eassumption.
+    + assumption.
+    + assumption.
 Qed.
 
 Theorem equivalence_query_execution_spec v1 v2 smt :
@@ -1148,52 +856,6 @@ Theorem equivalence_query_sat_correct v1 v2 smt ρ :
     v1 (SMT.execution_of_valuation TaggedVariable.VerilogLeft (SMT.nameMap smt) ρ)
     v2 (SMT.execution_of_valuation TaggedVariable.VerilogRight (SMT.nameMap smt) ρ).
 Proof. intros. now apply equivalence_query_execution_spec. Qed.
-
-Definition match_map_execution tag (m : VerilogSMTBijection.t) (e : execution) :=
-  forall var,
-    (exists smtName, m (tag, var) = Some smtName) <-> (exists xbv, e var = Some xbv).
-
-Lemma execution_of_valuation_left_match_on (m : VerilogSMTBijection.t) e1 e2 l :
-  RegisterState.defined_value_for (fun var => In var l) e1 ->
-  SMT.match_map_vars TaggedVariable.VerilogLeft m l ->
-  SMT.execution_of_valuation TaggedVariable.VerilogLeft m
-    (SMT.valuation_of_executions m e1 e2) =( l )= e1.
-Proof.
-  unfold SMT.execution_of_valuation, SMT.valuation_of_executions.
-  (* intros Hdefined Hexists var Hvar_in. *)
-  intros Hdefined Hmatch var Hvar_in.
-  pose proof Hvar_in as H.
-  apply Hmatch in H. destruct H as [smtName HsmtName].
-  rewrite HsmtName.
-  rewrite VerilogSMTBijection.bij_wf in HsmtName.
-  rewrite HsmtName.
-  apply Hdefined in Hvar_in. destruct Hvar_in as [bv Hbv].
-  rewrite Hbv, XBV.xbv_bv_inverse.
-  autodestruct; [|contradiction].
-  rewrite <- eq_rect_eq.
-  reflexivity.
-Qed.
-
-Lemma execution_of_valuation_right_match_on (m : VerilogSMTBijection.t) e1 e2 l :
-  RegisterState.defined_value_for (fun var => In var l) e2 ->
-  SMT.match_map_vars TaggedVariable.VerilogRight m l ->
-  SMT.execution_of_valuation TaggedVariable.VerilogRight m
-    (SMT.valuation_of_executions m e1 e2) =( l )= e2.
-Proof.
-  unfold SMT.execution_of_valuation, SMT.valuation_of_executions.
-  (* intros Hdefined Hexists var Hvar_in. *)
-  intros Hdefined Hmatch var Hvar_in.
-  pose proof Hvar_in as H.
-  apply Hmatch in H. destruct H as [smtName HsmtName].
-  rewrite HsmtName.
-  rewrite VerilogSMTBijection.bij_wf in HsmtName.
-  rewrite HsmtName.
-  apply Hdefined in Hvar_in. destruct Hvar_in as [bv Hbv].
-  rewrite Hbv, XBV.xbv_bv_inverse.
-  autodestruct; [|contradiction].
-  rewrite <- eq_rect_eq.
-  reflexivity.
-Qed.
 
 Lemma limit_to_regs_rewrite vars e1 e2 :
   (forall var, In var vars -> e1 var = e2 var) ->
@@ -1282,30 +944,6 @@ Proof.
   - rewrite Hmatch_outputs. assumption.
 Qed.
 
-Lemma match_map_execution_map_equal (m1 m2 : VerilogSMTBijection.t) tag e:
-  (forall n, m1 (tag, n) = m2 (tag, n)) ->
-  match_map_execution tag m1 e <-> match_map_execution tag m2 e.
-Proof.
-  intros.
-  unfold match_map_execution.
-  setoid_rewrite H.
-  reflexivity.
-Qed.
-
-Lemma verilog_to_smt_match_map_execution tag start v s e :
-  VerilogToSMT.verilog_to_smt tag start v = inr s ->
-  exact_execution v e ->
-  match_map_execution tag (SMT.nameMap s) e.
-Proof.
-  unfold match_map_execution, exact_execution.
-  intros Hfunc Hexact.
-  pose proof VerilogToSMTCorrect.verilog_to_smt_map_match as Hmap_vars.
-  insterU Hmap_vars.
-  unfold SMT.match_map_vars in *.
-  intros ?.
-  etransitivity; eauto.
-Qed.
-
 Lemma valid_execution_all_vars_defined tag start v q e :
   VerilogToSMT.verilog_to_smt tag start v = inr q ->
   valid_execution v e ->
@@ -1360,7 +998,7 @@ Proof.
   - eassumption.
   - eassumption.
   - setoid_rewrite inputs_outputs_subset.
-    eapply execution_of_valuation_right_match_on; [|assumption].
+    eapply SMT.execution_of_valuation_right_match_on; [|assumption].
     (* defined_value_for right-tagged vars *)
     destruct Hcounterexample as [? [? [[Hinputs_match Hinputs_defined] ?]]].
     eapply valid_execution_all_vars_defined; eauto.
@@ -1368,7 +1006,7 @@ Proof.
     rewrite inputs_match in Hinputs_defined.
     apply Hinputs_defined.
   - setoid_rewrite inputs_outputs_subset.
-    eapply execution_of_valuation_left_match_on; [|assumption].
+    eapply SMT.execution_of_valuation_left_match_on; [|assumption].
     (* defined_value_for left-tagged vars *)
     destruct Hcounterexample as [? [? [[Hinputs_match Hinputs_defined] ?]]].
     eapply valid_execution_all_vars_defined; eauto.
