vera/VerilogToSMT/Match.v
@@ -36,58 +36,15 @@ Import SigTNotations.
 
 Local Open Scope list.
 
-Inductive verilog_smt_match_value {w} : XBV.xbv w -> SMTLib.value -> Prop :=
-| verilog_smt_match_value_intro bv :
-  verilog_smt_match_value (XBV.from_bv bv) (SMTLib.Value_BitVec w bv).
-
-Definition verilog_smt_match_to_bv n (xbv : XBV.xbv n) (bv : BV.bitvector n):
-  XBV.to_bv xbv = Some bv ->
-  verilog_smt_match_value xbv (SMTLib.Value_BitVec n bv).
-Proof.
-  intros H.
-  apply XBV.bv_xbv_inverse in H.
-  subst xbv.
-  constructor.
-Qed.
-
-Definition verilog_smt_match_to_bv_bits
-  n1 n2 (xbv : XBV.xbv n1) (bv1 : BV.bitvector n1) (bv2 : BV.bitvector n2):
-  XBV.to_bv xbv = Some bv1 ->
-  BV.bits bv1 = BV.bits bv2 ->
-  verilog_smt_match_value xbv (SMTLib.Value_BitVec n2 bv2).
-Proof.
-  destruct bv1 as [bv1 wf1], bv2 as [bv2 wf2]. simpl. intros H1 H2.
-  apply XBV.bv_xbv_inverse in H1.
-  subst.
-  constructor.
-Qed.
-
-Definition valuation_has_var tag (m : VerilogSMTBijection.t) ρ var : Prop :=
-  exists smtName bv,
-    m (tag, var) = Some smtName /\
-      ρ smtName = Some (SMTLib.Value_BitVec (Verilog.varType var) bv).
-
-Inductive verilog_smt_match_on_name (regs : RegisterState.t) (ρ : SMTQueries.valuation) var smtName : Prop :=
-| verilog_smt_match_on_names_intro val
-    (Hsmtval : ρ smtName = Some val)
-    (Hmatchvals : verilog_smt_match_value (regs var) val).
-
-(* TODO: No longer used, deleteme *)
-Definition verilog_smt_match_states
-  (tag : TaggedVariable.Tag)
-  (m : VerilogSMTBijection.t)
-  (regs : RegisterState.t)
-  (ρ : SMTQueries.valuation) : Prop :=
-  forall verilogName smtName,
-    m (tag, verilogName) = Some smtName ->
-    verilog_smt_match_on_name regs ρ verilogName smtName.
-
+Definition verilog_smt_match_on_name (regs : RegisterState.t) (ρ : SMTLib.valuation) var smtName : Prop :=
+  regs var = XBV.from_bv (ρ (SMTLib.Sort_BitVec (Verilog.varType var)) smtName).
+    
 Definition verilog_smt_match_states_partial
   (cond : Verilog.variable -> Prop)
   (tag : TaggedVariable.Tag)
   (m : VerilogSMTBijection.t)
   (regs : RegisterState.t)
-  (ρ : SMTQueries.valuation) : Prop :=
+  (ρ : SMTLib.valuation) : Prop :=
   forall var,
     cond var ->
     exists smtName,
@@ -113,23 +70,16 @@ Proof.
   crush.
 Qed.
 
-Lemma verilog_smt_match_states_execution_of_valuation_same C tag (m : VerilogSMTBijection.t) ρ :
-  (forall var, C var -> valuation_has_var tag m ρ var) ->
-  verilog_smt_match_states_partial C tag m (SMT.execution_of_valuation tag m ρ) ρ.
+Lemma verilog_smt_match_states_execution_of_valuation_same tag (m : VerilogSMTBijection.t) ρ :
+  verilog_smt_match_states_partial (fun var => exists smtName, m (tag, var) = Some smtName) tag m (SMT.execution_of_valuation tag m ρ) ρ.
 Proof.
   intros Hhas_var.
   unfold verilog_smt_match_states_partial, SMT.execution_of_valuation.
-  intros var HC.
-  edestruct Hhas_var as [smtName [bv [HsmtName HsmtVal]]]; eauto.
+  intros [smtName HsmtName].
   exists smtName. split; [eassumption|].
-  econstructor.
-  - eassumption.
-  - rewrite HsmtName.
-    rewrite HsmtVal.
-    autodestruct; [|contradiction].
-    f_equal.
-    rewrite <- eq_rect_eq.
-    constructor.
+  unfold verilog_smt_match_on_name.
+  rewrite HsmtName.
+  reflexivity.
 Qed.
 
 Lemma verilog_smt_match_states_partial_impl P1 P2 tag m regs ρ :
@@ -145,20 +95,20 @@ Lemma verilog_smt_match_states_partial_set_reg_out C tag m r ρ var val :
 Proof.
   intro Hcond1.
   unfold verilog_smt_match_states_partial.
+  unfold verilog_smt_match_on_name in *.
   split; intros H * Hcond2.
   - destruct (dec (var0 = var)).
     + subst. contradiction.
-    + insterU H. destruct H as [smtName [? []]].
+    + insterU H. destruct H as [smtName [? Hverilogval]].
       econstructor. split. { eassumption. }
-      rewrite RegisterState.set_reg_get_out in Hmatchvals by congruence.
-      econstructor; eassumption.
+      rewrite RegisterState.set_reg_get_out in Hverilogval by congruence.
+      assumption.
   - destruct (dec (var0 = var)).
     + subst. contradiction.
-    + insterU H. destruct H as [smtName [? []]].
+    + insterU H. destruct H as [smtName [? Hverilogval]].
       econstructor. split. { eassumption. }
-      econstructor; try eassumption; [idtac].
       rewrite RegisterState.set_reg_get_out by congruence.
-      eassumption.
+      assumption.
 Qed.
 
 Lemma verilog_smt_match_states_partial_split C1 C2 C3 tag m reg ρ :
@@ -181,29 +131,26 @@ Proof. unfold verilog_smt_match_states_partial. crush. Qed.
 
 Lemma verilog_smt_match_states_partial_set_reg_elim C tag (m : VerilogSMTBijection.t) regs ρ var bv :
   (exists smtName,
-      m (tag, var) = Some smtName /\ ρ smtName = Some (SMTLib.Value_BitVec _ bv)) ->
+      m (tag, var) = Some smtName /\ ρ (SMTLib.Sort_BitVec (Verilog.varType var)) smtName = bv) ->
   verilog_smt_match_states_partial C tag m regs ρ ->
   verilog_smt_match_states_partial C tag m (RegisterState.set_reg var (XBV.from_bv bv) regs) ρ.
 Proof.
   unfold verilog_smt_match_states_partial.
+  unfold verilog_smt_match_on_name.
   intros Hvar Hrest *.
   destruct (dec (var0 = var)); intros Hcond.
   - subst.
     insterU Hvar. destruct Hvar as [? [? ?]].
-    insterU Hrest. destruct Hrest as [? [? []]].
+    insterU Hrest. destruct Hrest as [? [? ?]].
     replace x0 with x in * by congruence.
-    inv Hmatchvals.
-    repeat econstructor; try eassumption; [idtac].
+    repeat econstructor; try eassumption; expect 1.
     rewrite RegisterState.set_reg_get_in.
     repeat f_equal.
-    rewrite H0 in Hsmtval.
-    inv Hsmtval. constructor.
+    congruence.
   - insterU Hvar. destruct Hvar as [? [? ?]].
-    insterU Hrest. destruct Hrest as [? [? []]].
-    inv Hmatchvals.
-    repeat econstructor; try eassumption; [idtac].
+    insterU Hrest. destruct Hrest as [? [? ?]].
+    repeat econstructor; try eassumption; expect 1.
     rewrite RegisterState.set_reg_get_out; eauto.
-    rewrite <- H3. constructor.
 Qed.
 
 Lemma verilog_smt_match_states_partial_change_regs C tag m r1 r2 ρ :
@@ -214,11 +161,11 @@ Proof.
   unfold verilog_smt_match_states_partial.
   intros Hsame Hmatch1 * Hcond.
   insterU Hsame. insterU Hcond. insterU Hmatch1.
-  destruct Hmatch1 as [smtName [? []]].
+  destruct Hmatch1 as [smtName [? ?]].
   exists smtName.
   split. { eassumption. }
-  econstructor; try eassumption; [idtac].
-  rewrite <- Hsame. assumption.
+  unfold verilog_smt_match_on_name in *.
+  congruence.
 Qed.
 
 Ltac unpack_verilog_smt_match_states_partial :=
@@ -238,12 +185,9 @@ Lemma verilog_smt_match_states_partial_defined_value_for C tag m regs ρ :
   verilog_smt_match_states_partial C tag m regs ρ ->
   RegisterState.defined_value_for C regs.
 Proof.
-  unfold verilog_smt_match_states_partial, RegisterState.defined_value_for.
+  unfold verilog_smt_match_states_partial, verilog_smt_match_on_name, RegisterState.defined_value_for.
   intros Hmatch * Hcond.
-  insterU Hmatch.
-  destruct Hmatch as [? [? []]].
-  inv Hmatchvals.
-  eauto.
+  edestruct Hmatch as [? [? ?]]; eauto.
 Qed.
 
 Lemma verilog_smt_match_states_partial_execution_match_on C tag m ρ e :
@@ -251,14 +195,11 @@ Lemma verilog_smt_match_states_partial_execution_match_on C tag m ρ e :
     e ={ C }= SMT.execution_of_valuation tag m ρ.
 Proof.
   unfold verilog_smt_match_states_partial, "_ ={ _ }= _".
+  unfold verilog_smt_match_on_name.
   intros H var Hvar.
   edestruct H as [? [H1 H2]]; [eauto|].
-  inv H2. inv Hmatchvals.
   unfold SMT.execution_of_valuation.
-  rewrite H1, Hsmtval.
-  autodestruct; [|contradiction].
-  rewrite <- eq_rect_eq.
-  crush.
+  rewrite H1. assumption.
 Qed.
 
 Lemma verilog_smt_match_states_partial_execution_defined_value_for C tag m ρ e :
@@ -268,9 +209,34 @@ Proof.
   unfold verilog_smt_match_states_partial, RegisterState.defined_value_for.
   intros H var Hvar.
   edestruct H as [? [H1 H2]]; [eauto|].
-  inv H2. inv Hmatchvals.
-  eauto.
+  inv H2. eauto.
 Qed.
+
+Lemma execution_of_valuation_inv tag m ρ var bv :
+  SMT.execution_of_valuation tag m ρ var = XBV.from_bv bv ->
+  exists smtName,
+    m (tag, var) = Some smtName /\
+    ρ (SMTLib.Sort_BitVec (Verilog.varType var)) smtName = bv .
+Proof.
+  unfold SMT.execution_of_valuation.
+  intros H.
+  (* We don't know that var is in m. We could have added it directly
+  as an assumption, but we can also deduce it from the fact that the
+  value of the var in e is defined. This is only possible, however, if
+  the var is not zero-width (because zero-width Xs are
+  indistinguishable from zero-width 0/1s). This lemma is why we have
+  added varTypeWf into verilog variables *)
+
+  destruct (m (tag, var)).
+  - apply XBV.from_bv_injective in H.
+    eauto.
+  - exfalso.
+    apply f_equal with (f:=XBV.to_bv) in H.
+    autorewrite with xbv in H.
+    rewrite XBV.exes_to_bv in H by apply Verilog.varTypeWf.
+    discriminate.
+Qed.
+
 
 Lemma execution_match_on_verilog_smt_match_states_partial C tag m ρ e :
     RegisterState.defined_value_for C e ->
@@ -281,18 +247,23 @@ Proof.
   intros Hdefined Heq var Hvar.
   insterU Hdefined. insterU Heq.
   destruct Hdefined as [bv Hbv]. 
-  rewrite Hbv in Heq.
-  unfold SMT.execution_of_valuation in Heq.
-  (* The problem is with 0-length Xs. They look identical to 0-length non-Xs *)
-  autodestruct_eqn E.
-  all: apply f_equal with (f:=XBV.to_bv) in Heq.
-  all: assert (Verilog.varType var > 0)%N by admit.
-  all: autorewrite with xbv in Heq.
-  all: try discriminate; expect 1.
-  subst. simpl in *.
-  autorewrite with xbv in Heq. inv Heq.
-  eexists. split; [reflexivity|].
-  econstructor; eauto.
-  rewrite Hbv.
-  constructor.
-Admitted.
+  unfold verilog_smt_match_on_name in *.
+  unfold SMT.execution_of_valuation in *.
+
+  (* TODO: Use execution_of_valuation_inv instead. *)
+
+  (* We don't know that var is in m. We could have added it directly
+  as an assumption, but we can also deduce it from the fact that the
+  value of the var in e is defined. This is only possible, however, if
+  the var is not zero-width (because zero-width Xs are
+  indistinguishable from zero-width 0/1s). This lemma is why we have
+  added varTypeWf into verilog variables *)
+
+  destruct (m (tag, var)); [solve [eauto]|].
+  exfalso.
+  rewrite Hbv in Heq. clear Hbv.
+  apply f_equal with (f:=XBV.to_bv) in Heq.
+  autorewrite with xbv in Heq.
+  rewrite XBV.exes_to_bv in Heq by apply Verilog.varTypeWf.
+  discriminate.
+Qed.
